CppFormalization/Cpp2/Closure/External/All.lean
@@ -1,3 +1,7 @@
+import CppFormalization.Cpp2.Closure.External.AdequacyContractsV3
+import CppFormalization.Cpp2.Closure.External.AdequacyKernelV3
+import CppFormalization.Cpp2.Closure.External.AdequacyNormalV3
+import CppFormalization.Cpp2.Closure.External.AdequacyReturnV3
 import CppFormalization.Cpp2.Closure.External.AlignmentV3
 import CppFormalization.Cpp2.Closure.External.AssembleLemmasV3
 import CppFormalization.Cpp2.Closure.External.AssembleV3
@@ -9,8 +13,11 @@ import CppFormalization.Cpp2.Closure.External.GlueV3
 import CppFormalization.Cpp2.Closure.External.Interface
 import CppFormalization.Cpp2.Closure.External.InterfaceV2
 import CppFormalization.Cpp2.Closure.External.InterfaceV3
+import CppFormalization.Cpp2.Closure.External.LegacyBridgeV2
+import CppFormalization.Cpp2.Closure.External.LegacyBridgeV3
 import CppFormalization.Cpp2.Closure.External.LegacyBuilderV3
 import CppFormalization.Cpp2.Closure.External.ObjectDeclRuntimeBridgeV3
+--import CppFormalization.Cpp2.Closure.External.ObjectDeclStdFragmentV3
 import CppFormalization.Cpp2.Closure.External.ReadyAssemblyV3
 import CppFormalization.Cpp2.Closure.External.ReadyFromGlueV3
 import CppFormalization.Cpp2.Closure.External.ReflectionFragmentV2
@@ -21,7 +28,14 @@ import CppFormalization.Cpp2.Closure.External.SplitBuilderV3
 import CppFormalization.Cpp2.Closure.External.StdFragmentV2
 import CppFormalization.Cpp2.Closure.External.StdFragmentV3
 import CppFormalization.Cpp2.Closure.External.ToyBuilderV3
+import CppFormalization.Cpp2.Closure.External.ToyGlueInstanceV3
 import CppFormalization.Cpp2.Closure.External.ToyReadyInstanceV3
 import CppFormalization.Cpp2.Closure.External.ToySplitBuilderV3
 import CppFormalization.Cpp2.Closure.External.TransportPropsV3
 import CppFormalization.Cpp2.Closure.External.TransportV3
+
+/-!
+# Closure.External.All
+
+Build-coverage aggregate for `Closure.External`.
+-/
